allocator/slabs bottom-up 12/n
size_class vprop: almost done

src/SizeClass.fst
@@ -8,6 +8,8 @@ module U8 = FStar.UInt8
 open FStar.Ghost
 
 module SL = Selectors.LList
+//friend Selectors.LList
+
 open Steel.FractionalPermission
 module Mem = Steel.Memory
 open Steel.Effect.Atomic
@@ -19,10 +21,51 @@ module A = Steel.Array
 open Utils2
 open SlabsUtils
 
+#push-options "--ide_id_info_off"
+
+noextract
+let is_empty
+  (size_class: sc)
+  (s: Seq.lseq U64.t 4)
+  : prop
+  =
+  let max = FStar.Int.max_int U64.n in
+  let bound = U32.v (nb_slots size_class) / 64 in
+  (U64.v (Seq.index s 0) = 0) /\
+  (bound > 1 && (U64.v (Seq.index s 1) = 0)) /\
+  (bound > 2 && (U64.v (Seq.index s 2) = 0)) /\
+  (bound > 3 && (U64.v (Seq.index s 3) = 0))
+
+noextract
+let has_free_slot
+  (size_class: sc)
+  (s: Seq.lseq U64.t 4)
+  : bool
+  =
+  let max = FStar.Int.max_int U64.n in
+  let bound = U32.v (nb_slots size_class) / 64 in
+  (U64.v (Seq.index s 0) < max) ||
+  (bound > 1 && (U64.v (Seq.index s 1) < max)) ||
+  (bound > 2 && (U64.v (Seq.index s 2) < max)) ||
+  (bound > 3 && (U64.v (Seq.index s 3) < max))
+
+noextract
+let has_nonfree_slot
+  (size_class: sc)
+  (s: Seq.lseq U64.t 4)
+  : bool
+  =
+  let bound = U32.v (nb_slots size_class) / 64 in
+  (U64.v (Seq.index s 0) > 0) ||
+  (bound > 1 && (U64.v (Seq.index s 1) > 0)) ||
+  (bound > 2 && (U64.v (Seq.index s 2) > 0)) ||
+  (bound > 3 && (U64.v (Seq.index s 3) > 0))
+
 assume val f (md: slab_metadata) : arr:array U8.t{A.length arr = U32.v page_size}
 
 [@@ __reduce__]
-unfold let p (size_class: sc)
+//unfold
+let p (size_class: sc)
   =
   fun (md: slab_metadata)
   ->
@@ -30,16 +73,12 @@ unfold let p (size_class: sc)
   slab_vprop size_class (f md) 0 (U32.v (nb_slots size_class)))
 
 [@@ __reduce__]
-unfold let p_empty (size_class: sc)
+//unfold
+let p_empty (size_class: sc)
   =
   fun (md: slab_metadata)
   ->
-  (A.varray md `vrefine`
-    (fun s ->
-      Seq.index s 0 = 0UL /\
-      Seq.index s 1 = 0UL /\
-      Seq.index s 2 = 0UL /\
-      Seq.index s 3 = 0UL))
+  (A.varray md `vrefine` (fun s -> is_empty size_class s))
   `star`
   slab_vprop size_class (f md) 0 (U32.v (nb_slots size_class))
 
@@ -56,50 +95,62 @@ type size_class_struct = {
 noeq
 type blob = {
   scs_v: size_class_struct;
-  partial_slabs_v: SL.t slab_metadata;
-  empty_slabs_v: SL.t slab_metadata;
+  partial_slabs_v: list slab_metadata;
+  empty_slabs_v: list slab_metadata;
 }
 
 let size_class_sl'
   (r: ref size_class_struct)
-  (blob: blob)
+  (scs: size_class_struct)
   : Mem.slprop u#1
   =
-  pts_to_sl r full_perm (blob.scs_v) `Mem.star`
-  pts_to_sl (blob.scs_v.partial_slabs) full_perm (blob.partial_slabs_v) `Mem.star`
-  //SL.ind_llist_sl (p_empty blob.scs_v.size) (blob.scs_v.empty_slabs)
-  pts_to_sl (blob.scs_v.empty_slabs) full_perm (blob.empty_slabs_v)
+  pts_to_sl r full_perm scs `Mem.star`
+  SL.ind_llist_sl (p_empty scs.size) (scs.partial_slabs) `Mem.star`
+  SL.ind_llist_sl (p_empty scs.size) (scs.empty_slabs)
 
 let size_class_sl
   (r: ref size_class_struct)
   =
   Mem.h_exists (size_class_sl' r)
 
+let size_class_sl'_witinv (r: ref size_class_struct)
+  : Lemma (Mem.is_witness_invariant (size_class_sl' r))
+  =
+  let aux (scs1 scs2: size_class_struct) (m: Mem.mem)
+  : Lemma
+  (requires
+    Mem.interp (size_class_sl' r scs1) m /\
+    Mem.interp (size_class_sl' r scs2) m
+  )
+  (ensures scs1 == scs2)
+  =
+  pts_to_witinv r full_perm;
+  assert (scs1 == scs2);
+  pts_to_witinv (scs1.partial_slabs) full_perm;
+  pts_to_witinv (scs1.empty_slabs) full_perm
+  in
+  Classical.forall_intro_3 (Classical.move_requires_3 aux)
+
 let size_class_sel_full'
   (r: ref size_class_struct)
   : selector' blob (size_class_sl r)
   =
-  fun h ->
-    let b = Mem.id_elim_exists (size_class_sl' r) h in
+  fun (h:_) ->
+    let scs : size_class_struct = reveal (Mem.id_elim_exists (size_class_sl' r) h) in
+    assert (Mem.interp (size_class_sl' r scs) h);
+    let p1 = pts_to_sl r full_perm scs in
+    let p2 = SL.ind_llist_sl (p_empty scs.size) scs.partial_slabs in
+    let p3 = SL.ind_llist_sl (p_empty scs.size) scs.empty_slabs in
+    let sl = p1 `Mem.star` p2 `Mem.star` p3 in
+    assert (Mem.interp sl h);
+    let partial_slabs_v = SL.ind_llist_sel (p_empty scs.size) scs.partial_slabs h in
+    let empty_slabs_v = SL.ind_llist_sel (p_empty scs.size) scs.empty_slabs h in
+    let b = {
+      scs_v = reveal scs;
+      partial_slabs_v = partial_slabs_v;
+      empty_slabs_v = empty_slabs_v;
+    } in
     b
-
-let size_class_sl'_witinv (r: ref size_class_struct)
-  : Lemma (Mem.is_witness_invariant (size_class_sl' r))
-  =
-  let aux (b1 b2: blob) (m: Mem.mem)
-  : Lemma
-  (requires
-    Mem.interp (size_class_sl' r b1) m /\
-    Mem.interp (size_class_sl' r b2) m
-  )
-  (ensures b1 == b2)
-  =
-  pts_to_witinv r full_perm;
-  assert (b1.scs_v == b2.scs_v);
-  pts_to_witinv (b1.scs_v.partial_slabs) full_perm;
-  pts_to_witinv (b1.scs_v.empty_slabs) full_perm
-  in
-  Classical.forall_intro_3 (Classical.move_requires_3 aux)
 
 let size_class_sel_depends_only_on
   (r: ref size_class_struct)
@@ -158,17 +209,18 @@ let unpack_sc_lemma
   (ensures (
     Mem.interp (
       SR.ptr r `Mem.star`
-      SR.ptr (b.scs_v.partial_slabs) `Mem.star`
-      SR.ptr (b.scs_v.empty_slabs)
+      SL.ind_llist_sl (p_empty b.scs_v.size) b.scs_v.partial_slabs `Mem.star`
+      SL.ind_llist_sl (p_empty b.scs_v.size) b.scs_v.empty_slabs
     ) m /\
     sel_of (vptr r) m == b.scs_v /\
-    sel_of (vptr b.scs_v.partial_slabs) m == b.partial_slabs_v /\
-    sel_of (vptr b.scs_v.empty_slabs) m == b.empty_slabs_v
+    SL.ind_llist_sel (p_empty b.scs_v.size) b.scs_v.partial_slabs m == b.partial_slabs_v /\
+    SL.ind_llist_sel (p_empty b.scs_v.size) b.scs_v.empty_slabs m == b.empty_slabs_v /\
+    True
   ))
   =
   let p1 = pts_to_sl r full_perm b.scs_v in
-  let p2 = pts_to_sl (b.scs_v.partial_slabs) full_perm (b.partial_slabs_v) in
-  let p3 = pts_to_sl (b.scs_v.empty_slabs) full_perm (b.empty_slabs_v) in
+  let p2 = SL.ind_llist_sl (p_empty b.scs_v.size) b.scs_v.partial_slabs in
+  let p3 = SL.ind_llist_sl (p_empty b.scs_v.size) b.scs_v.empty_slabs in
   let sl = p1 `Mem.star` p2 `Mem.star` p3 in
   assert (Mem.interp sl m);
 
@@ -179,37 +231,34 @@ let unpack_sc_lemma
   ptr_sel_interp r m1;
   pts_to_witinv r full_perm;
   // #2
-  intro_ptr_interp (b.scs_v.partial_slabs) (b.partial_slabs_v) m2;
-  ptr_sel_interp (b.scs_v.partial_slabs) m2;
-  pts_to_witinv (b.scs_v.partial_slabs) full_perm;
   // #3
-  intro_ptr_interp (b.scs_v.empty_slabs) (b.empty_slabs_v) m3;
-  ptr_sel_interp (b.scs_v.empty_slabs) m3;
-  pts_to_witinv (b.scs_v.empty_slabs) full_perm;
+  //
   Mem.intro_star
-    (SR.ptr r)
-    (SR.ptr (b.scs_v.partial_slabs)) m1 m2;
+    (SR.ptr r) p2 m1 m2;
   assert (reveal m12 == Mem.join m1 m2);
   Mem.intro_star
-    (SR.ptr r `Mem.star` SR.ptr (b.scs_v.partial_slabs))
-    (SR.ptr (b.scs_v.empty_slabs)) m12 m3;
+    (SR.ptr r `Mem.star` p2) p3 m12 m3;
   assert (m == Mem.join m12 m3);
-  //@2
-  admit ()
+  ()
 
-
+#push-options "--z3rlimit 30"
 let unpack_sc (r: ref size_class_struct)
   : Steel size_class_struct
   (size_class_full r)
   (fun scs ->
     vptr r `star`
-    vptr scs.partial_slabs `star`
-    vptr scs.empty_slabs
+    SL.ind_llist (p_empty scs.size) scs.partial_slabs `star`
+    SL.ind_llist (p_empty scs.size) scs.empty_slabs
+    //SL.ind_llist_sel (p_empty b.scs_v.size) b.scs_v.partial_slabs m == b.partial_slabs_v /\
+    //SL.ind_llist_sel (p_empty b.scs_v.size) b.scs_v.empty_slabs m == b.empty_slabs_v /\
   )
   (requires fun _ -> True)
   (ensures fun h0 scs h1 ->
     let b = v_sc_full r h0 in
     sel r h1 == scs /\
+    //TODO
+    //SL.v_ind_llist (p_empty scs.size) scs.partial_slabs h1 == b.partial_slabs_v /\
+    //SL.v_ind_llist (p_empty scs.size) scs.empty_slabs h1 == b.empty_slabs_v /\
     True
     //@2 b.scs_v.partial_slabs == sel scs.partial_slabs h1 /\
     //@2 b.scs_v.empty_slabs == sel scs.empty_slabs h1
@@ -220,53 +269,77 @@ let unpack_sc (r: ref size_class_struct)
   change_slprop
     (size_class_full r)
     (vptr r `star`
-    vptr b.scs_v.partial_slabs `star`
-    vptr b.scs_v.empty_slabs)
+    SL.ind_llist (p_empty b.scs_v.size) b.scs_v.partial_slabs `star`
+    SL.ind_llist (p_empty b.scs_v.size) b.scs_v.empty_slabs)
     b
     ((b.scs_v, b.partial_slabs_v), b.empty_slabs_v)
     (fun m -> unpack_sc_lemma r (reveal b) m);
   let scs = read r in
   change_slprop_rel
-    (vptr b.scs_v.partial_slabs)
-    (vptr scs.partial_slabs)
+    (SL.ind_llist (p_empty b.scs_v.size) b.scs_v.partial_slabs)
+    (SL.ind_llist (p_empty scs.size) scs.partial_slabs)
     (fun x y -> x == y)
     (fun _ -> ());
   change_slprop_rel
-    (vptr b.scs_v.empty_slabs)
-    (vptr scs.empty_slabs)
+    (SL.ind_llist (p_empty b.scs_v.size) b.scs_v.empty_slabs)
+    (SL.ind_llist (p_empty scs.size) scs.empty_slabs)
     (fun x y -> x == y)
     (fun _ -> ());
   return scs
 
 let pack_sc_lemma
   (r: ref size_class_struct)
+  (scs: size_class_struct)
   (b: blob)
   (m: Mem.mem)
   : Lemma
   (requires
     Mem.interp (
       SR.ptr r `Mem.star`
-      SR.ptr (b.scs_v.partial_slabs) `Mem.star`
-      SR.ptr (b.scs_v.empty_slabs)
+      SL.ind_llist_sl (p_empty scs.size) scs.partial_slabs `Mem.star`
+      SL.ind_llist_sl (p_empty scs.size) scs.empty_slabs
     ) m /\
     sel_of (vptr r) m == b.scs_v /\
-    sel_of (vptr b.scs_v.partial_slabs) m == b.partial_slabs_v /\
-    sel_of (vptr b.scs_v.empty_slabs) m == b.empty_slabs_v
+    SL.ind_llist_sel (p_empty scs.size) scs.partial_slabs m == b.partial_slabs_v /\
+    SL.ind_llist_sel (p_empty scs.size) scs.empty_slabs m == b.empty_slabs_v /\
+    True
+    //sel_of (vptr b.scs_v.partial_slabs) m == b.partial_slabs_v /\
+    //sel_of (vptr b.scs_v.empty_slabs) m == b.empty_slabs_v
   )
-  (ensures (
+  (ensures
     Mem.interp (size_class_sl r) m /\
     size_class_sel r m == b
-  ))
+  )
   =
-  admit ()
+  admit ();
+  let p1 = SR.ptr r in
+  let p2 = SL.ind_llist_sl (p_empty b.scs_v.size) b.scs_v.partial_slabs in
+  let p3 = SL.ind_llist_sl (p_empty b.scs_v.size) b.scs_v.empty_slabs in
+  let sl = p1 `Mem.star` p2 `Mem.star` p3 in
+  assert (Mem.interp sl m);
+
+  let m12, m3 = Mem.id_elim_star (p1 `Mem.star` p2) p3 m in
+  Mem.join_commutative m12 m3;
+  let m1, m2 = Mem.id_elim_star p1 p2 m12 in
+  Mem.join_commutative m1 m2;
+  // #1
+  ptr_sel_interp r m1;
+  // #2
+  // #3
+  //
+  Mem.intro_star p1 p2 m1 m2;
+  assert (reveal m12 == Mem.join m1 m2);
+  Mem.intro_star (p1 `Mem.star` p2) p3 m12 m3;
+  assert (m == Mem.join m12 m3);
+  ()
 
 let pack_sc (#opened:_)
   (r: ref size_class_struct)
   (scs: size_class_struct)
   : SteelGhost unit opened
   (vptr r `star`
-  vptr scs.partial_slabs `star`
-  vptr scs.empty_slabs)
+  SL.ind_llist (p_empty scs.size) scs.partial_slabs `star`
+  SL.ind_llist (p_empty scs.size) scs.empty_slabs)
   (fun _ -> size_class_full r)
   (requires fun h0 -> sel r h0 == scs)
   (ensures fun _ _ _ ->
@@ -274,19 +347,33 @@ let pack_sc (#opened:_)
     True)
   =
   let h0 = get () in
-  let b : erased blob = hide ({
+  assert (scs == sel r h0);
+  let partial_slabs_v : list slab_metadata =
+    hide (SL.v_ind_llist (p_empty scs.size) scs.partial_slabs h0) in
+  let empty_slabs_v : list slab_metadata =
+    hide (SL.v_ind_llist (p_empty scs.size) scs.empty_slabs h0) in
+  //let m : erased ((size_class_struct * list slab_metadata) * list slab_metadata)
+  //= hide ((scs, reveal partial_slabs_v), reveal empty_slabs_v) in
+  let m2 : erased ((size_class_struct * list slab_metadata) * list slab_metadata)
+  = gget (vptr r `star`
+  SL.ind_llist (p_empty scs.size) scs.partial_slabs `star`
+  SL.ind_llist (p_empty scs.size) scs.empty_slabs) in
+  //assert (m == m2);
+  //admit ();
+  let b : blob = hide ({
     scs_v = scs;
-    partial_slabs_v = sel scs.partial_slabs h0;
-    empty_slabs_v = sel scs.empty_slabs h0;
+    partial_slabs_v = reveal partial_slabs_v;
+    empty_slabs_v = reveal empty_slabs_v;
   }) in
   change_slprop
     (vptr r `star`
-    vptr b.scs_v.partial_slabs `star`
-    vptr b.scs_v.empty_slabs)
+    SL.ind_llist (p_empty scs.size) scs.partial_slabs `star`
+    SL.ind_llist (p_empty scs.size) scs.empty_slabs)
     (size_class_full r)
-    ((b.scs_v, b.partial_slabs_v), b.empty_slabs_v)
+    m2
     b
-    (fun m -> pack_sc_lemma r (reveal b) m)
+    (fun m -> admit (); pack_sc_lemma r scs (reveal b) m);
+  ()
 
 // TODO
 // - intermediate step with lemmas in order to have packing/unpacking
